autoclrs/ch31-number-theory/CLRS.Ch31.ExtendedGCD.ImplTest.fsti
@@ -1,0 +1,8 @@
+module CLRS.Ch31.ExtendedGCD.ImplTest
+
+open Pulse.Lib.Pervasives
+open FStar.SizeT
+
+module SZ = FStar.SizeT
+
+val test_extended_gcd (_:unit) : stt bool emp (fun r -> pure (r == true))
